pausing progress on this; time to write a quals document that doesn't use any of it...

src/AAI/Lang/Arith.v
@@ -1,72 +1,293 @@
-Inductive lang :=
-  | Num : nat -> lang
-  | Times : lang -> lang -> lang.
+Require Import FP.Core.
+Require Import FP.Data.Nat.
+Require Import FP.Data.String.
+Require Import FP.Data.ListSet.
+Require Import FP.Data.Bool.
+Require Import FP.Data.WF.
+Require Import FP.Data.Unit.
+Require Import FP.Data.Prop.
+Require Import FP.Data.PSet.
+Require Import FP.Classes.Lattice.
+Require Import FP.Classes.Monad.
+Require Import FP.Classes.MGalois.
 
-Inductive abstract :=
-  | Top
-  | Even
-  | Odd
-  | Box.
-
-Fixpoint is_even (n:nat) : bool :=
-  match n with
-  | O => true
-  | S n' => negb (is_even n')
+Inductive v_lang :=
+  | v_Halt : v_lang
+  | v_Times : dom nat -> v_lang -> v_lang.
+Definition lang := lib v_lang.
+Definition Halt : dom lang := v_Halt.
+Definition Times : dom (nat ⇒ lang ⇒ lang) := λ n l → (v_Times : dom nat -> dom lang -> dom lang) n l.
+Fixpoint _lang_elim {A} (l:dom lang) : dom (A ⇒ (nat ⇒ A ⇒ A) ⇒ A) := λ h t →
+  match l with
+  | v_Halt => h
+  | v_Times n l => t ∙ n ∙ (_lang_elim l ∙ h ∙ t)
   end.
-Fixpoint is_evenp (n:nat) : Prop :=
-  match n with
-  | O => True
-  | S n' => not (is_evenp n')
-  end.
-
-Parameter joins : list abstract -> abstract.
-Parameter lte : abstract -> abstract -> Prop.
-Parameter map : forall {A B}, (A -> B) -> list A -> list B.
-Parameter lin : forall {A}, A -> list A -> Prop.
-  
-(* Standard Galois; can't build gamma *)
-Definition alpha (c:list nat) : abstract :=
-  joins (map (fun n => 
-    match is_even n with
-    | true => Even
-    | false => Odd
-    end) c).
-
-Definition gamma (a:abstract) : list nat.
-Abort.
-
-(* using Prop to represent sets, not what we want *)
-Definition alpha' (c:nat -> Prop) : abstract -> Prop :=
-  fun a => 
-    match a with
-    | Top => True
-    | Even => forall x, c x -> is_evenp x
-    | Odd => forall x, c x -> not (is_evenp x)
-    | Bot => False
+Definition lang_elim {A} : dom (lang ⇒ A ⇒ (nat ⇒ A ⇒ A) ⇒ A) := λ l → _lang_elim l.
+Global Opaque Halt.
+Global Opaque Times.
+Global Opaque lang_elim.
+Ltac lang_induction e :=
+  induction e ;
+  repeat
+    match goal with
+    | H : context [v_Halt] |- _ => change v_Halt with Halt in H
+    | H : context [v_Times ?n ?l] |- _ => change (v_Times n l) with (Times ∙ n ∙ l) in H
+    | |- context [v_Halt] => change v_Halt with Halt
+    | |- context [v_Times ?n ?l] => change (v_Times n l) with (Times ∙ n ∙ l)
     end.
-Definition gamma' (a:abstract -> Prop) : nat -> Prop :=
-  fun n =>
-    match is_even n with
-    | true => forall x, a x -> lte x Even
-    | false => forall x, a x -> lte x Odd
-    end.
-
-Definition falpha' (c:(nat -> Prop) -> (nat -> Prop)) : (abstract -> Prop) -> abstract -> Prop :=
-  fun f => alpha' (c (gamma' f)).
-Definition fgamma' (a:(abstract -> Prop) -> (abstract -> Prop)) : (nat -> Prop) -> nat -> Prop :=
-  fun f => gamma' (a (alpha' f)).
-
-(* using a weaker notion of galois *)
-Definition galois (c:list nat) (a:abstract) : Prop :=
-  match a with
-  | Top => True
-  | Even => forall x, lin x c -> is_evenp x
-  | Odd => forall x, lin x c -> not (is_evenp x)
-  | Bot => False
+Definition lang_elim_beta_Halt {A} (h:dom A) (t:dom (nat ⇒ A ⇒ A)) 
+: lang_elim ∙ Halt ∙ h ∙ t ≃ h := libReflexivity.
+Definition lang_elim_beta_Times {A} (h:dom A) (t:dom (nat ⇒ A ⇒ A)) n l 
+: lang_elim ∙ (Times ∙ n ∙ l) ∙ h ∙ t ≃ t ∙ n ∙ (lang_elim ∙ l ∙ h ∙ t) := libReflexivity.
+Definition lang_elim_eta (e:dom lang) : lang_elim ∙ e ∙ Halt ∙ Times ≃ e.
+Proof.
+  lang_induction e.
+  - LibReflexivity.
+  - change (Times ∙ d ∙ (lang_elim ∙ e ∙ Halt ∙ Times) ≃ Times ∙ d ∙ e).
+    qproper_elim.
+Qed.
+Ltac LangRewrite :=
+  match goal with
+  | |- ⟨ lang_elim ∙ Halt ∙ ?h ∙ ?t IN _ |_| _ ⟩ => ReplaceBy (lang_elim_beta_Halt h t)
+  | |- ⟨ lang_elim ∙ (Times ∙ ?n ∙ ?l) ∙ ?h ∙ ?t IN _ |_| _ ⟩ => ReplaceBy (lang_elim_beta_Times h t n l)
+  | |- ⟨ lang_elim ∙ ?e ∙ Halt ∙ Times IN _ |_| _ ⟩ => ReplaceBy (lang_elim_eta e)
   end.
 
-Definition fgalois (cf:list nat -> list nat) (af:abstract -> abstract) : Prop :=
-  forall c a, galois c a -> galois (cf c) (af a).
-  
-  
-  
+Inductive v_abstract :=
+  | v_Top
+  | v_Even
+  | v_Odd
+  | v_Bot.
+Inductive v_abstract_lte : relation v_abstract :=
+  | BotLte : forall a, v_abstract_lte v_Bot a
+  | TopLte : forall a, v_abstract_lte a v_Top.
+Instance : Eqv v_abstract := lib_Eqv.
+Instance : Lte v_abstract := { lte := v_abstract_lte }.
+Admitted.
+Definition abstract := {| qdom := v_abstract |}.
+Definition Top : dom abstract := v_Top.
+Definition Even : dom abstract := v_Even.
+Definition Odd : dom abstract := v_Odd.
+Definition Bot : dom abstract := v_Bot.
+Definition abstract_elim {A} 
+: dom (abstract ⇒ (unit ⇒ A) ⇒ (unit ⇒ A) ⇒ (unit ⇒ A) ⇒ (unit ⇒ A) ⇒ A) := λ a t e o b →
+    match a : dom abstract with
+    | v_Top => t ∙ tt
+    | v_Even => e ∙ tt
+    | v_Odd => o ∙ tt
+    | v_Bot => b ∙ tt
+    end.
+Global Opaque Top.
+Global Opaque Even.
+Global Opaque Odd.
+Global Opaque Bot.
+Global Opaque abstract_elim.
+Ltac abstract_induction e :=
+  induction e ;
+  repeat
+    match goal with
+    | H : context [v_Top] |- _ => change v_Top with Top in H
+    | H : context [v_Even] |- _ => change v_Even with Even in H
+    | H : context [v_Odd] |- _ => change v_Odd with Odd in H
+    | H : context [v_Bot] |- _ => change v_Bot with Bot in H
+    | |- context [v_Top] => change v_Top with Top
+    | |- context [v_Even] => change v_Even with Even
+    | |- context [v_Odd] => change v_Odd with Odd
+    | |- context [v_Bot] => change v_Bot with Bot
+    end.
+Definition abstract_elim_beta_Top {A} t e o b
+: abstract_elim (A:=A) ∙ Top ∙ t ∙ e ∙ o ∙ b ≃ t ∙ tt := libReflexivity.
+Definition abstract_elim_beta_Even {A} t e o b
+: abstract_elim (A:=A) ∙ Even ∙ t ∙ e ∙ o ∙ b ≃ e ∙ tt := libReflexivity.
+Definition abstract_elim_beta_Odd {A} t e o b
+: abstract_elim (A:=A) ∙ Odd ∙ t ∙ e ∙ o ∙ b ≃ o ∙ tt := libReflexivity.
+Definition abstract_elim_beta_Bot {A} t e o b
+: abstract_elim (A:=A) ∙ Bot ∙ t ∙ e ∙ o ∙ b ≃ b ∙ tt := libReflexivity.
+Ltac AbstractRewrite :=
+  match goal with
+  | |- ⟨ abstract_elim ∙ Top ∙ ?t ∙ ?e ∙ ?o ∙ ?b IN _ |_| _ ⟩ => ReplaceBy (abstract_elim_beta_Top t e o b)
+  | |- ⟨ abstract_elim ∙ Even ∙ ?t ∙ ?e ∙ ?o ∙ ?b IN _ |_| _ ⟩ => ReplaceBy (abstract_elim_beta_Even t e o b)
+  | |- ⟨ abstract_elim ∙ Odd ∙ ?t ∙ ?e ∙ ?o ∙ ?b IN _ |_| _ ⟩ => ReplaceBy (abstract_elim_beta_Odd t e o b)
+  | |- ⟨ abstract_elim ∙ Bot ∙ ?t ∙ ?e ∙ ?o ∙ ?b IN _ |_| _ ⟩ => ReplaceBy (abstract_elim_beta_Bot t e o b)
+  end.
+                                                  
+Inductive v_alang :=
+  | v_AHalt : v_alang
+  | v_ATimes : dom abstract -> v_alang -> v_alang.
+Inductive v_alang_lte : relation v_alang :=
+  | AHaltLte : v_alang_lte v_AHalt v_AHalt
+  | ATimesLte : forall a₁ a₂ l, a₁ ⊑ a₂ -> v_alang_lte (v_ATimes a₁ l) (v_ATimes a₂ l).
+Instance : Eqv v_alang := lib_Eqv.
+Instance : Lte v_alang := { lte := v_alang_lte }.
+Admitted.
+Definition alang := {| qdom := v_alang |}.
+Definition AHalt : dom alang := v_AHalt.
+Definition ATimes : dom (abstract ⇒ alang ⇒ alang) := λ a al → 
+  (v_ATimes : dom abstract -> dom alang -> dom alang) a al.
+Fixpoint _alang_elim {A} (al:dom alang)  : dom (A ⇒ (abstract ⇒ A ⇒ A) ⇒ A) := λ hp fp →
+  match al with
+  | v_AHalt => hp
+  | v_ATimes a al => fp ∙ a $ _alang_elim al ∙ hp ∙ fp
+  end.
+Definition alang_elim {A} : dom (alang ⇒ A ⇒ (abstract ⇒ A ⇒ A) ⇒ A) := λ a → _alang_elim a.
+Global Opaque AHalt.
+Global Opaque ATimes.
+Global Opaque alang_elim.
+Ltac alang_induction e :=
+  induction e ; 
+  repeat
+    match goal with
+    | H : context [v_AHalt] |- _ => change v_AHalt with AHalt in H
+    | H : context [v_ATimes ?a ?al] |- _ => change (v_ATimes a al) with (ATimes ∙ a ∙ al) in H
+    | |- context [v_AHalt] => change v_AHalt with AHalt
+    | |- context [v_ATimes ?a ?al] => change (v_ATimes a al) with (ATimes ∙ a ∙ al)
+    end.
+Definition alang_elimM {m A} `{! Monad m } : dom (alang ⇒ A ⇒ (abstract ⇒ A ⇒ m A) ⇒ m A) := λ a hp tp →
+  alang_elim ∙ a ∙ (ret ∙ hp) ∙ (λ a r → tp ∙ a =<< r).
+Definition alang_elim_beta_AHalt {A} (h:dom A) (f:dom (abstract ⇒ A ⇒ A))
+: alang_elim ∙ AHalt ∙ h ∙ f ≃ h := libReflexivity.
+Definition alang_elim_beta_ATimes {A} (h:dom A) (f:dom (abstract ⇒ A ⇒ A)) a al
+: alang_elim ∙ (ATimes ∙ a ∙ al) ∙ h ∙ f ≃ f ∙ a ∙ (alang_elim ∙ al ∙ h ∙ f) := libReflexivity.
+Definition alang_elim_eta (e:dom alang) : alang_elim ∙ e ∙ AHalt ∙ ATimes ≃ e.
+Proof.
+  alang_induction e.
+  - LibReflexivity.
+  - change (ATimes ∙ d ∙ (alang_elim ∙ e ∙ AHalt ∙ ATimes) ≃ ATimes ∙ d ∙ e).
+    qproper_elim.
+Qed.
+Ltac AlangRewrite :=
+  match goal with
+  | |- ⟨ alang_elim ∙ AHalt ∙ ?h ∙ ?f IN _ |_| _ ⟩ => ReplaceBy (alang_elim_beta_AHalt h f)
+  | |- ⟨ alang_elim ∙ (ATimes ∙ ?a ∙ ?al) ∙ ?h ∙ ?f IN _ |_| _ ⟩ => ReplaceBy (alang_elim_beta_ATimes h f a al)
+  | |- ⟨ alang_elim ∙ ?e ∙ AHalt ∙ ATimes IN _ |_| _ ⟩ => ReplaceBy (alang_elim_eta e)
+  end.
+
+Instance : Lattice alang.
+Admitted.
+
+Definition decEven : dom (nat ⇒ bool) := undefined.
+
+Inductive v_isEven : dom nat -> Prop :=
+  | ZEven : v_isEven vZ
+  | SEven : forall n, v_isEven n -> v_isEven (vS (vS n)).
+Inductive v_isOdd : dom nat -> Prop :=
+  | ZOdd : v_isOdd (vS vZ)
+  | SOdd : forall n, v_isOdd n -> v_isOdd (vS (vS n)).
+
+Definition isEven : dom (nat ⇒ prop) := λ n → v_isEven n : dom prop.
+Definition isOdd : dom (nat ⇒ prop) := λ n → v_isOdd n : dom prop.
+
+Definition αnat : dom (nat ⇒ abstract) := λ n →
+  case ∙ (decEven ∙ n) ∙ (λ _ → Even) ∙ (λ _ → Odd).
+Definition γTop : dom (wfT listSet nat) := wfT_fix $ λ γTop →
+  ret ∙ Z m+ ret ∙ (S ∙ γTop).
+Definition γTop2 : dom (pset nat) := suniversal.
+
+Definition γEven : dom (wfT listSet nat) := wfT_fix $ λ γEven →
+  ret ∙ Z m+ ret ∙ (S $ S ∙ γEven).
+Definition γEven2 : dom (pset nat) := PSet ∙ isEven.
+
+Definition γOdd : dom (wfT listSet nat) := wfT_fix $ λ γOdd →
+  ret ∙ (S ∙ Z) m+ ret ∙ (S $ S ∙ γOdd).
+Definition γOdd2 : dom (pset nat) := PSet ∙ isOdd.
+
+Definition γnat : dom (abstract ⇒ wfT listSet nat) := λ a →
+  abstract_elim ∙ a
+    ∙ (λ _ → γTop)
+    ∙ (λ _ → γEven)
+    ∙ (λ _ → γOdd)
+    ∙ (λ _ → mzero).
+
+Instance : MGalois (wfT listSet) nat abstract :=
+  { mgaloisα := kret ∙ αnat
+  ; mgaloisγ := γnat
+  }.
+Proof.
+  - qproper_elim.
+    Re fail || match goal with |- ⟨ y IN _ |_| _ ⟩ => StrengthenBy H end.
+    clear H y.
+    abstract_induction x ; Re fail || AbstractRewrite.
+    + admit.
+    + unfold γEven.
+      EnterLeft ; PushFun ; PushArg.
+      match goal with |- ⟨ wfT_fix ∙ ?f IN _ |_| _ ⟩ => ReplaceBy (wfT_fix_beta f) end.
+      PopArg ; PopFun ; ExitLeft.
+      Re fail || MonadRewrite.
+      simpl.
+    + admit.
+    + admit.
+  - admit.
+Defined.
+
+(* (nat -> Prop) -> nat -> anat
+
+
+     abs : nat -> anat
+     conc : anat -> nat -> Prop
+
+     forall n, conc (abs n) n     (soundness)
+     forall a, (forall n, (conc a) n -> abs n = a)
+
+     step_conc : nat -> nat
+     step_abs  : anat -> anat
+
+     1. forall n, abs (step_conc n) <= step_abs (abs n)
+     2. forall a, (forall n, conc a n -> 
+                      abs (conc_step n) <= abs_step a)
+*)
+
+
+
+Definition αlang : dom (lang ⇒ alang) := λ l →
+  lang_elim ∙ l ∙ AHalt $ λ n al → ATimes ∙ (αnat ∙ n) ∙ al.
+Definition αlangM : dom (lang ⇒ wfT listSet alang) := kret ∙ αlang.
+Definition γlangM : dom (alang ⇒ wfT listSet lang) := λ a →
+  alang_elimM ∙ a ∙ Halt $ λ a l → 
+    n ← γnat ∙ a ;;
+    ret $ Times ∙ n ∙ l.
+
+Section MGalois.
+  Instance : MGalois (wfT listSet) lang alang :=
+    { mgaloisα := αlangM
+    ; mgaloisγ := γlangM
+    }.
+  Proof.
+    - Local Opaque αnat.
+      Local Opaque γnat.
+      Local Opaque γlangM.
+      apply qmonotonic_intro ; unfold "⇉" ; intros ; simpl.
+      Re fail || match goal with |- ⟨ y IN _ |_| _ ⟩ => StrengthenBy H end.
+      clear H y.
+      alang_induction x ; Re fail || LangRewrite || AlangRewrite || MonadRewrite.
+      EnterLeft.
+ Admitted.
+End MGalois.
+      (*
+      ReplaceBy (bind_associativity (A:=abstract) (alang_elim ∙  _ αlangM).
+      MonadRewrite.
+      PushFun.
+      PushArg.
+      apply (lte_replace_lte IHx).
+      WeakenBy IHx.
+      Re fail || WeakenBy IHx.
+      idtac.
+      match goal with
+      | IHx : ?t |- _ => assert t
+      end.
+      Re fail || LangRewrite || AlangRewrite || MonadRewrite.
+      epose (_=IHx).
+      eapply IHx.
+      + simpl.
+      match goal with
+      | |- context E[ alang_elimM ∙ ?e ∙ _ ∙ _ ] => eapply alang_indM (typeof E) _ _ 
+      Re fail || MonadRewrite.
+      Re fail || match goal with |- ⟨ x IN _ |LTE| _ ⟩ => WeakenBy H end.
+      EnterLeft.
+      PushFun.
+      PushArg.
+      PushFun.
+      PushFun.
+      PushArg.
+      apply (replaceBy H).
+      simpl.
+*)
