src/FP/Core/Rewrite.v
@@ -2,6 +2,7 @@ Require Import FP.Core.Relations.
 Require Import FP.Core.Universe.
 Require Import FP.Core.QType.
 Require Import FP.Core.Tactic.
+Require Import FP.Core.Notation.
 
 Definition topk {A} : dom (A ⇒ A) := id.
 Definition focusFun {A B C} (x:dom A) (k:dom (B ⇒ C)) : dom ((A ⇒ B) ⇒ C) :=
@@ -21,106 +22,106 @@ Definition state {A B:qtype} (m:mode) :=
 Opaque state.
 
 Notation "⊤κ" := topk.
-Infix "◁" := focusFun (at level 60, right associativity).
-Infix "▷" := focusArg (at level 60, right associativity).
-Notation "⟨ x ∈ k | m | y ⟩" := (state m x k y).
+Infix "◁" := focusFun.
+Infix "▷" := focusArg.
+Notation "⟨ x 'IN' k | m | y ⟩" := (state m x k y).
 
 Ltac EnterLeft :=
   match goal with
-  | |- ?x ≃ ?y => change ⟨ x ∈ ⊤κ |EQV| y ⟩
-  | |- ?x ⊑ ?y => change ⟨ x ∈ ⊤κ |LTE| y ⟩
+  | |- ?x ≃ ?y => change ⟨ x IN ⊤κ |EQV| y ⟩
+  | |- ?x ⊑ ?y => change ⟨ x IN ⊤κ |LTE| y ⟩
   end.
 Ltac ExitLeft :=
   match goal with
-  | |- ⟨ ?x ∈ ⊤κ |EQV| ?y ⟩ => change (x ≃ y)
-  | |- ⟨ ?x ∈ ⊤κ |LTE| ?y ⟩ => change (x ⊑ y)
+  | |- ⟨ ?x IN ⊤κ |EQV| ?y ⟩ => change (x ≃ y)
+  | |- ⟨ ?x IN ⊤κ |LTE| ?y ⟩ => change (x ⊑ y)
   end.
 Ltac EnterRight :=
   match goal with
-  | |- ?x ≃ ?y => Symmetry ; change ⟨ y ∈ ⊤κ |EQV| x ⟩
-  | |- ?x ⊑ ?y => change ⟨ y ∈ ⊤κ |GTE| x ⟩
+  | |- ?x ≃ ?y => Symmetry ; change ⟨ y IN ⊤κ |EQV| x ⟩
+  | |- ?x ⊑ ?y => change ⟨ y IN ⊤κ |GTE| x ⟩
   end.
 Ltac ExitRight :=
   match goal with
-  | |- ⟨ ?y ∈ ⊤κ |EQV| ?x ⟩ => change (y ≃ x) ; Symmetry
-  | |- ⟨ ?y ∈ ⊤κ |GTE| ?x ⟩ => change (x ⊑ y)
+  | |- ⟨ ?y IN ⊤κ |EQV| ?x ⟩ => change (y ≃ x) ; Symmetry
+  | |- ⟨ ?y IN ⊤κ |GTE| ?x ⟩ => change (x ⊑ y)
   end.
 
 Ltac PushFun :=
   match goal with
-  | |- ⟨ ?f ∙ ?x ∈ ?k |EQV| ?y ⟩ => change ⟨ f ∈ (x ◁ k) |EQV| y ⟩
-  | |- ⟨ ?f ∙ ?x ∈ ?k |LTE| ?y ⟩ => change ⟨ f ∈ (x ◁ k) |LTE| y ⟩
-  | |- ⟨ ?f ∙ ?x ∈ ?k |GTE| ?y ⟩ => change ⟨ f ∈ (x ◁ k) |GTE| y ⟩
+  | |- ⟨ ?f ∙ ?x IN ?k |EQV| ?y ⟩ => change ⟨ f IN (x ◁ k) |EQV| y ⟩
+  | |- ⟨ ?f ∙ ?x IN ?k |LTE| ?y ⟩ => change ⟨ f IN (x ◁ k) |LTE| y ⟩
+  | |- ⟨ ?f ∙ ?x IN ?k |GTE| ?y ⟩ => change ⟨ f IN (x ◁ k) |GTE| y ⟩
   end.
 Ltac PopFun :=
   match goal with
-  | |- ⟨ ?f ∈ (?x ◁ ?k) |EQV| ?y ⟩ => change ⟨ f ∙ x ∈ k |EQV| y ⟩
-  | |- ⟨ ?f ∈ (?x ◁ ?k) |LTE| ?y ⟩ => change ⟨ f ∙ x ∈ k |LTE| y ⟩
-  | |- ⟨ ?f ∈ (?x ◁ ?k) |GTE| ?y ⟩ => change ⟨ f ∙ x ∈ k |GTE| y ⟩
+  | |- ⟨ ?f IN (?x ◁ ?k) |EQV| ?y ⟩ => change ⟨ f ∙ x IN k |EQV| y ⟩
+  | |- ⟨ ?f IN (?x ◁ ?k) |LTE| ?y ⟩ => change ⟨ f ∙ x IN k |LTE| y ⟩
+  | |- ⟨ ?f IN (?x ◁ ?k) |GTE| ?y ⟩ => change ⟨ f ∙ x IN k |GTE| y ⟩
   end.
 Ltac PushArg :=
   match goal with
-  | |- ⟨ ?f ∙ ?x ∈ ?k |EQV| ?y ⟩ => change ⟨ x ∈ (f ▷ k) |EQV| y ⟩
-  | |- ⟨ ?f ∙ ?x ∈ ?k |LTE| ?y ⟩ => change ⟨ x ∈ (f ▷ k) |LTE| y ⟩
-  | |- ⟨ ?f ∙ ?x ∈ ?k |GTE| ?y ⟩ => change ⟨ x ∈ (f ▷ k) |GTE| y ⟩
+  | |- ⟨ ?f ∙ ?x IN ?k |EQV| ?y ⟩ => change ⟨ x IN (f ▷ k) |EQV| y ⟩
+  | |- ⟨ ?f ∙ ?x IN ?k |LTE| ?y ⟩ => change ⟨ x IN (f ▷ k) |LTE| y ⟩
+  | |- ⟨ ?f ∙ ?x IN ?k |GTE| ?y ⟩ => change ⟨ x IN (f ▷ k) |GTE| y ⟩
   end.
 Ltac PopArg :=
   match goal with
-  | |-  ⟨ ?x ∈ (?f ▷ ?k) |EQV| ?y ⟩ => change ⟨ f ∙ x ∈ k |EQV| y ⟩
-  | |-  ⟨ ?x ∈ (?f ▷ ?k) |LTE| ?y ⟩ => change ⟨ f ∙ x ∈ k |LTE| y ⟩
-  | |-  ⟨ ?x ∈ (?f ▷ ?k) |GTE| ?y ⟩ => change ⟨ f ∙ x ∈ k |GTE| y ⟩
+  | |-  ⟨ ?x IN (?f ▷ ?k) |EQV| ?y ⟩ => change ⟨ f ∙ x IN k |EQV| y ⟩
+  | |-  ⟨ ?x IN (?f ▷ ?k) |LTE| ?y ⟩ => change ⟨ f ∙ x IN k |LTE| y ⟩
+  | |-  ⟨ ?x IN (?f ▷ ?k) |GTE| ?y ⟩ => change ⟨ f ∙ x IN k |GTE| y ⟩
   end.
 
 Definition eqv_replace {A B} {x x':dom A} {k:dom (A ⇒ B)} {y:dom B} 
-(e:x ≃ x') (g:⟨ x' ∈ k |EQV| y ⟩) : ⟨ x ∈ k |EQV| y ⟩.
+(e:x ≃ x') (g:⟨ x' IN k |EQV| y ⟩) : ⟨ x IN k |EQV| y ⟩.
 Proof.
   change (k ∙ x ≃ y).
   Transitivity (k ∙ x') ; qproper_elim.
   exact g.
 Qed.
 Definition lte_replace_lte {A B} {x x':dom A} {k:dom (A ⇒ B)} {y:dom B}
-(e:x ⊑ x') (g:⟨ x' ∈ k |LTE| y ⟩) : ⟨ x ∈ k |LTE| y ⟩.
+(e:x ⊑ x') (g:⟨ x' IN k |LTE| y ⟩) : ⟨ x IN k |LTE| y ⟩.
 Proof.
   change (k ∙ x ⊑ y).
   Transitivity (k ∙ x') ; qproper_elim.
   exact g.
 Qed.
 Definition lte_replace_eqv {A B} {x x':dom A} {k:dom (A ⇒ B)} {y:dom B}
-(e:x ≃ x') : ⟨ x' ∈ k |LTE| y ⟩ -> ⟨ x ∈ k |LTE| y ⟩ := lte_replace_lte (reflexivity e).
+(e:x ≃ x') : ⟨ x' IN k |LTE| y ⟩ -> ⟨ x IN k |LTE| y ⟩ := lte_replace_lte (reflexivity e).
 Definition gte_replace_gte {A B} {x x':dom A} {k:dom (A ⇒ B)} {y:dom B}
-(d:x' ⊑ x) (g:⟨ x' ∈ k |GTE| y ⟩) : ⟨ x ∈ k |GTE| y ⟩.
+(d:x' ⊑ x) (g:⟨ x' IN k |GTE| y ⟩) : ⟨ x IN k |GTE| y ⟩.
 Proof.
   change (y ⊑ k ∙ x).
   Transitivity (k ∙ x') ; qproper_elim.
   exact g.
 Qed.
 Definition gte_replace_eqv {A B} {x x':dom A} {k:dom (A ⇒ B)} {y:dom B}
-(e:x ≃ x') : ⟨ x' ∈ k |GTE| y ⟩ -> ⟨ x ∈ k |GTE| y ⟩ := 
+(e:x ≃ x') : ⟨ x' IN k |GTE| y ⟩ -> ⟨ x IN k |GTE| y ⟩ := 
   gte_replace_gte (reflexivity (symmetry e)).
 Ltac ReplaceBy p :=
   match goal with
-  | |- ⟨ ?x ∈ ?k |EQV| ?y ⟩ => apply (eqv_replace p)
-  | |- ⟨ ?x ∈ ?k |LTE| ?y ⟩ => apply (lte_replace_eqv p)
-  | |- ⟨ ?x ∈ ?k |GTE| ?y ⟩ => apply (gte_replace_eqv p)
+  | |- ⟨ ?x IN ?k |EQV| ?y ⟩ => apply (eqv_replace p)
+  | |- ⟨ ?x IN ?k |LTE| ?y ⟩ => apply (lte_replace_eqv p)
+  | |- ⟨ ?x IN ?k |GTE| ?y ⟩ => apply (gte_replace_eqv p)
   end.
 Ltac WeakenBy p :=
   match goal with
-  | |- ⟨ ?x ∈ ?k |LTE| ?y ⟩ => apply (lte_replace_lte p)
+  | |- ⟨ ?x IN ?k |LTE| ?y ⟩ => apply (lte_replace_lte p)
   end.
 Ltac StrengthenBy p :=
   match goal with
-  | |- ⟨ ?x ∈ ?k |GTE| ?y ⟩ => apply (gte_replace_gte p)
+  | |- ⟨ ?x IN ?k |GTE| ?y ⟩ => apply (gte_replace_gte p)
   end.
 
 Ltac Everywhere_k t :=
-  match goal with
-  | |- ⟨ _ ∙ _ ∈ _ | _ | _ ⟩ =>
-      chain PushFun ; Everywhere_k t ; PopFun |+|
-      chain PushArg ; Everywhere_k t ; PopArg |+|
-      t ; repeat t
-  | _ => t ; repeat t
-  end.
+  chain
+    (match goal with
+    |- ⟨ _ ∙ _ IN _ | _ | _ ⟩ =>
+        chain PushFun ; Everywhere_k t ; PopFun |+|
+        PushArg ; Everywhere_k t ; PopArg
+    end || fail) |+|
+  (t ; repeat t).
 Ltac Everywhere t :=
   try (EnterLeft ; Everywhere_k t ; ExitLeft) ;
   try (EnterRight ; Everywhere_k t ; ExitRight).
-Tactic Notation "Re" tactic2(t) := Everywhere t.
+Tactic Notation "Re" tactic2(t) := repeat (Everywhere t ; qproper_elim).
