src/FP/Classes/Galois.v
@@ -3,21 +3,21 @@ Require Import FP.Core.
 Class Galois (A B:qtype) :=
   { galoisα : dom (A ⇒ B)
   ; galoisγ : dom (B ⇒ A)
-  ; galois_id_αγ : (galoisα ⊙ galoisγ) ⊑ id
-  ; galois_id_γα : id ⊑ (galoisγ ⊙ galoisα)
+  ; galois_id_αγ : galoisα ⊙ galoisγ ⊑ id
+  ; galois_id_γα : id ⊑ galoisγ ⊙ galoisα
   }.
 Global Opaque galoisα.
 Global Opaque galoisγ.
 
 Ltac GaloisRewrite :=
   match goal with
-  | |- ⟨ (galoisα (A:=?A) (B:=?B)) ⊙ (galoisγ (A:=?A) (B:=?B)) ∈ _ |LTE| _ ⟩ =>
+  | |- ⟨ (galoisα (A:=?A) (B:=?B)) ⊙ (galoisγ (A:=?A) (B:=?B)) IN _ |LTE| _ ⟩ =>
       WeakenBy (galois_id_αγ (A:=A) (B:=B))
-  | |- ⟨ galoisα ∙ (galoisγ ∙ ?e) ∈ _ |LTE| _ ⟩ => 
+  | |- ⟨ galoisα ∙ (galoisγ ∙ ?e) IN _ |LTE| _ ⟩ => 
       WeakenBy (qmonotonic_elim galois_id_αγ e e libReflexivity)
-  | |- ⟨ (galoisγ (A:=?A) (B:=?B)) ⊙ (galoisα (A:=?A) (B:=?B)) ∈ _ |GTE| _ ⟩ =>
+  | |- ⟨ (galoisγ (A:=?A) (B:=?B)) ⊙ (galoisα (A:=?A) (B:=?B)) IN _ |GTE| _ ⟩ =>
       StrengthenBy (galois_id_γα (A:=A) (B:=B))
-  | |- ⟨ galoisγ ∙ (galoisα ∙ ?e) ∈ _ |GTE| _ ⟩ =>
+  | |- ⟨ galoisγ ∙ (galoisα ∙ ?e) IN _ |GTE| _ ⟩ =>
       StrengthenBy (qmonotonic_elim galois_id_γα e e libReflexivity)
   end.
 
@@ -26,14 +26,6 @@ Instance : forall A B `{! Galois A B }, Galois (A ⇒ A) (B ⇒ B) :=
   ; galoisγ := λ g → galoisγ ⊙ g ⊙ galoisα
   }.
 Proof.
-  - qproper.
-    Transitivity (x ∙ (galoisα ∙ (galoisγ ∙ x0))).
-    + eapply (qmonotonic_elim galois_id_αγ) ; LibReflexivity.
-    + qproper_elim.
-      eapply (qmonotonic_elim galois_id_αγ) ; auto.
-  - qproper.
-    Transitivity (y ∙ (galoisγ ∙ (galoisα ∙ y0))).
-    + qproper_elim.
-      eapply (qmonotonic_elim galois_id_γα) ; auto.
-    + eapply (qmonotonic_elim galois_id_γα) ; LibReflexivity.
+  - Re fail || GaloisRewrite.
+  - Re fail || GaloisRewrite.
 Defined.
