src/FP/Classes/Lattice.v
@@ -1,0 +1,17 @@
+Require Import FP.Core.
+
+Class Lattice A :=
+  { top : dom A
+  ; bot : dom A
+  ; join : dom (A ⇒ A ⇒ A)
+  ; meet : dom (A ⇒ A ⇒ A)
+  ; join_left : forall x y, x ⊑ join ∙ x ∙ y
+  ; join_right : forall x y, y ⊑ join ∙ x ∙ y
+  ; meet_left : forall x y, meet ∙ x ∙ y ⊑ x
+  ; meet_right : forall x y, meet ∙ y ∙ x ⊑ y
+  }.
+
+Notation "⊤" := top.
+Notation "⊥" := bot.
+Notation "x ⊔ y" := (join ∙ x ∙ y).
+Notation "x ⊓ y" := (meet ∙ x ∙ y).
