src/FP/Classes/MGalois.v
@@ -1,0 +1,54 @@
+Require Import FP.Core.
+Require Import FP.Classes.Monad.
+Require Import FP.Classes.Galois.
+
+Class MGalois m `{! Monad m } (A B:qtype) :=
+  { mgaloisα : dom (A ⇒ m B)
+  ; mgaloisγ : dom (B ⇒ m A)
+  ; mgalois_id_αγ : mgaloisα m⊙ mgaloisγ ⊑ ret
+  ; mgalois_id_γα : ret ⊑ mgaloisγ m⊙ mgaloisα
+  }.
+Global Opaque mgaloisα.
+Global Opaque mgaloisγ.
+
+Ltac GaloisWFRewrite :=
+  match goal with
+  | |- ⟨ (mgaloisα (A:=?A) (B:=?B)) m⊙ (mgaloisγ (A:=?A) (B:=?B)) IN _ |LTE| _ ⟩ =>
+      WeakenBy (mgalois_id_αγ (A:=A) (B:=B))
+  | |- ⟨ (mgaloisγ ∙ ?e) >>= mgaloisα IN _ |LTE| _ ⟩ => 
+      WeakenBy (qmonotonic_elim mgalois_id_αγ e e libReflexivity)
+  | |- ⟨ (mgaloisγ (A:=?A) (B:=?B)) m⊙ (mgaloisα (A:=?A) (B:=?B)) IN _ |GTE| _ ⟩ =>
+      StrengthenBy (mgalois_id_γα (A:=A) (B:=B))
+  | |- ⟨ (mgaloisα ∙ ?e) >>= mgaloisγ IN _ |GTE| _ ⟩ =>
+      StrengthenBy (qmonotonic_elim mgalois_id_γα e e libReflexivity)
+  end.
+
+Section Galois1.
+  Local Opaque mcompose.
+  Instance : forall m A B `{! Monad m ,! MGalois m A B }, Galois (A ⇒ m A) (B ⇒ m B) :=
+    { galoisα := λ f → mgaloisα m⊙ f m⊙ mgaloisγ
+    ; galoisγ := λ g → mgaloisγ m⊙ g m⊙ mgaloisα
+    }.
+  Proof.
+    Local Ltac Hammer := Re fail || MonadRewrite || GaloisWFRewrite || KleisliRewrite.
+    - Hammer. 
+      Re fail || KleisliUnassoc ; Hammer.
+    - Hammer.
+      Re fail || KleisliUnassoc ; Hammer.
+  Defined.
+End Galois1.
+
+
+Section Galois2.
+  Instance : forall m A B `{! Monad m ,! MGalois m A B }, Galois (m A) (m B) :=
+    { galoisα := extend ∙ mgaloisα
+    ; galoisγ := extend ∙ mgaloisγ
+    }.
+  Proof.
+    Local Ltac Hammer := Re fail || MonadRewrite || GaloisWFRewrite.
+    - Hammer.
+      Transitivity (bind ∙ y ∙ ret) ; qproper_elim ; Hammer.
+    - Hammer.
+      Transitivity (bind ∙ x ∙ ret) ; qproper_elim ; Hammer.
+  Defined.
+End Galois2.
