src/FP/Classes/MTransition.v
@@ -1,0 +1,9 @@
+Require Import FP.Core.
+Require Import FP.Classes.Monad.
+Require Import FP.Classes.MGalois.
+
+Class MTransition m :=
+  { ss : qtype -> qtype
+  ; transition : forall A B, dom ((A ⇒ m B) ⇒ ss A ⇒ ss B)
+  ; transition_MGalois :> forall m' `{! Monad m' } A B, MGalois m' A B -> MGalois m' (ss A) (ss B)
+  }.
