src/FP/Classes/Sequence.v
@@ -1,0 +1,12 @@
+Require Import FP.Core.
+Require Import FP.Data.Stream.
+Require Import FP.Data.Nat.
+
+Class Compat (t:qtype -> qtype) := { compat : qtype -> Prop }.
+Arguments compat t {Compat} _.
+
+Class Sequence t `{! Compat t } :=
+  { toStream : forall {A}, compat t A -> dom (t A ⇒ stream A) 
+  ; fromStream : forall {A}, compat t A -> dom (stream A ⇒ t A)
+  ; length : forall {A}, compat t A -> dom (stream A ⇒ nat)
+  }.
