src/FP/Core/QType.v
@@ -1,6 +1,7 @@
 Require Import FP.Core.Relations.
 Require Import FP.Core.Universe.
 Require Import FP.Core.RFunction.
+Require Import FP.Core.Notation.
 
 Inductive qtype : Type := QType
   { qdom : Type
@@ -32,32 +33,25 @@ Definition flip_elim {τ} {x y:dom (dual τ)} (p:x ⊑ y) : (y:dom τ) ⊑ (x:do
 
 Definition hom (τ₁:qtype) (τ₂:qtype) : qtype :=
   {| qdom := dom τ₁ r⇒ dom τ₂ |}.
-Infix "⇒" := hom (at level 80, right associativity).
+Infix "⇒" := hom.
 
 Definition QMorphism {τ₁ τ₂:qtype} (f:dom τ₁ -> dom τ₂) (p:proper (eqv v⇉ eqv) f) (m:proper (lte v⇉ lte) f) 
 : dom (τ₁ ⇒ τ₂) := RFunction f p m.
 Definition QMorphismA {τ₁ τ₂:qtype} (f:dom τ₁ -> dom τ₂) : dom (τ₁ ⇒ τ₂).
 refine(QMorphism f _ _) ; admit.
 Defined.
-(*
-Notation "'λ'  x .. y → e" := 
-  (QMorphism (fun x => .. (QMorphism (fun y => e) _ _) ..) _ _)
-  (x binder, y binder, at level 200, right associativity).
-*)
-Notation "'λ'  x .. y → e" := 
-  (QMorphismA (fun x => .. (QMorphismA (fun y => e)) ..))
-  (x binder, y binder, at level 200, right associativity).
+Notation "'λ'  x .. y → e" := (QMorphismA (fun x => .. (QMorphismA (fun y => e)) ..)).
 
 
 Definition ap {τ₁ τ₂} : dom (τ₁ ⇒ τ₂) -> dom τ₁ -> dom τ₂ := rapply.
-Infix "∙" := ap (at level 20, left associativity).
-Infix "$" := ap (at level 99, right associativity, only parsing).
+Infix "∙" := ap.
+Infix "$" := ap (only parsing).
 
 Definition respectful {τ₁ τ₂} 
 (R1:relation (dom τ₁)) (R2:relation (dom τ₂)) (f g:dom (τ₁ ⇒ τ₂)) :=
   forall x y, R1 x y -> R2 (f ∙ x) (g ∙ y).
 Arguments respectful : simpl never.
-Infix "⇉" := respectful (at level 60, right associativity).
+Infix "⇉" := respectful.
 
 Definition qproper_intro {τ₁ τ₂} {f g:dom (τ₁ ⇒ τ₂)} (p:(eqv ⇉ eqv) f g) : eqv f g := p.
 Definition qproper_elim {τ₁ τ₂} {f g:dom (τ₁ ⇒ τ₂)} (p:eqv f g) : (eqv ⇉ eqv) f g := p.
@@ -93,14 +87,15 @@ Ltac qproper_elim :=
     repeat (
       qproper1 ||
       match goal with
-      | [ |- _ ∙ _ ≃ _ ∙ _ ] => apply qproper_apply
-      | [ |- _ ∙ _ ⊑ _ ∙ _ ] => apply qmonotonic_apply
+      | [ |- ?f ∙ ?x ≃ ?g ∙ ?y ] => apply (qproper_apply (f:=f) (g:=g) (x:=x) (y:=y))
+      | [ |- ?f ∙ ?x ⊑ ?g ∙ ?y ] => apply (qmonotonic_apply (f:=f) (g:=g) (x:=x) (y:=y))
       end)).
 
 Definition id {τ₁} : dom (τ₁ ⇒ τ₁) := λ x → x.
 Definition compose {τ₁ τ₂ τ₃} : dom ((τ₂ ⇒ τ₃) ⇒ (τ₁ ⇒ τ₂) ⇒ (τ₁ ⇒ τ₃)) :=
   λ g f x → g ∙ (f ∙ x).
-Notation "g ⊙ f" := (compose ∙ g ∙ f) (at level 60, right associativity).
+Notation "g ⊙ f" := (compose ∙ g ∙ f).
 Definition const {τ₁ τ₂} : dom (τ₁ ⇒ τ₂ ⇒ τ₁) := λ x _ → x.
 Definition applyTo {τ₁ τ₂} : dom (τ₁ ⇒ (τ₁ ⇒ τ₂) ⇒ τ₂) := λ x f → f ∙ x.
 Definition apply {τ₁ τ₂} : dom ((τ₁ ⇒ τ₂) ⇒ τ₁ ⇒ τ₂) := λ f x → f ∙ x.
+Definition on {A B C} : dom ((B ⇒ B ⇒ C) ⇒ (A ⇒ B) ⇒ (A ⇒ A ⇒ C)) := λ o f x y → o ∙ (f ∙ x) ∙ (f ∙ y).
