src/FP/Data/Bool.v
@@ -1,0 +1,42 @@
+Require Import FP.Core.
+Require Import FP.Data.Unit.
+Require Import FP.Classes.Lattice.
+
+Definition vbool := Coq.Init.Datatypes.bool.
+Definition vtrue := Coq.Init.Datatypes.true.
+Definition vfalse := Coq.Init.Datatypes.false.
+
+Definition bool := lib bool.
+Definition true : dom bool := vtrue.
+Definition false : dom bool := vfalse.
+Definition case {A} : dom (bool ⇒ (unit ⇒ A) ⇒ (unit ⇒ A) ⇒ A) := λ b t f →
+  if b : dom bool then t ∙ tt else f ∙ tt.
+Global Opaque true.
+Global Opaque false.
+Global Opaque case.
+Ltac bool_induction e :=
+  induction e ;
+  repeat
+    match goal with
+    | |- context[Coq.Init.Datatypes.true] => change Coq.Init.Datatypes.true with true
+    | |- context[Coq.Init.Datatypes.false] => change Coq.Init.Datatypes.false with false
+    end.
+  
+Definition and : dom (bool ⇒ bool ⇒ bool) := λ x y → case ∙ x ∙ (λ _ → y) ∙ (λ _ → false).
+
+Definition bool_beta_true {A} t f : case (A:=A) ∙ true ∙ t ∙ f ≃ t ∙ tt := libReflexivity.
+Definition bool_beta_false {A} t f : case (A:=A) ∙ false ∙ t ∙ f ≃ f ∙ tt := libReflexivity.
+Ltac BoolRewrite :=
+  match goal with
+  | |- ⟨ case ∙ true ∙ ?t ∙ ?f IN _ |_| _ ⟩ => ReplaceBy (bool_beta_true t f)
+  | |- ⟨ case ∙ false ∙ ?t ∙ ?f IN _ |_| _ ⟩ => ReplaceBy (bool_beta_false t f)
+  end.
+Definition bool_eta e : case ∙ e ∙ (λ _ → true) ∙ (λ _ → false) ≃ e.
+Proof.
+  bool_induction e ; Re fail || BoolRewrite.
+Qed.
+
+Definition bool_beta_lte {A} `{! Lattice A } e t f : case (A:=A) ∙ e ∙ t ∙ f ⊑ t ∙ tt ⊔ f ∙ tt.
+Proof.
+  bool_induction e ; Re fail || BoolRewrite ; apply join_left || apply join_right.
+Qed.
