src/FP/Data/Nat.v
@@ -1,0 +1,40 @@
+Require Import FP.Core.
+
+Definition vnat : Type := Coq.Init.Datatypes.nat.
+Definition vZ : nat := Coq.Init.Datatypes.O.
+Definition vS : nat -> nat := Coq.Init.Datatypes.S.
+                   
+Definition nat := lib vnat.
+Definition Z : dom nat := vZ.
+Definition S : dom (nat ⇒ nat) := λ n → (vS:dom nat -> dom nat) n.
+
+Fixpoint _nat_elim {A} (n:dom nat) : dom (A ⇒ (A ⇒ A) ⇒ A) := λ z s →
+  match n : dom nat with
+  | vZ => z : dom A
+  | vS n' => s $ _nat_elim n' ∙ z ∙ s
+  end.
+Definition nat_elim {A} : dom (nat ⇒ A ⇒ (A ⇒ A) ⇒ A) := λ a → _nat_elim a.
+Global Opaque Z.
+Global Opaque S.
+Global Opaque nat_elim.
+
+Ltac nat_induction e :=
+  induction e ;
+  repeat
+    match goal with
+    | H : context [Coq.Init.Datatypes.O] |- _ => change Coq.Init.Datatypes.O with Z in H
+    | H : context [Coq.Init.Datatypes.S ?n] |- _ => change (Coq.Init.Datatypes.S n) with (S ∙ n) in H
+    | |- context [Coq.Init.Datatypes.O] => change Coq.Init.Datatypes.O with Z
+    | |- context [Coq.Init.Datatypes.S ?n] => change (Coq.Init.Datatypes.S n) with (S ∙ n)
+    end.
+
+Definition nat_elim_beta_Z {A} z s : nat_elim (A:=A) ∙ Z ∙ z ∙ s ≃ z := libReflexivity.
+Definition nat_elim_beta_S {A} z s n : nat_elim (A:=A) ∙ (S ∙ n) ∙ z ∙ s ≃ s ∙ (nat_elim ∙ n ∙ z ∙ s) := libReflexivity.
+Ltac NatRewrite :=
+  match goal with
+  | |- ⟨ nat_elim ∙ Z ∙ ?z ∙ ?s IN _ |_| _ ⟩ => ReplaceBy (nat_elim_beta_Z z s)
+  | |- ⟨ nat_elim ∙ (S ∙ ?n) ∙ ?z ∙ ?s IN _ |_| _ ⟩ => ReplaceBy (nat_elim_beta_S z s n)
+  end.
+
+Definition pred : dom (nat ⇒ nat) := λ n →
+  nat_elim ∙ n ∙ Z ∙ id.
