src/FP/Data/PSet.v
@@ -1,0 +1,40 @@
+Require Import FP.Core.
+Require Import FP.Data.Prop.
+Require Import FP.Classes.Lattice.
+Require Import FP.Classes.Monad.
+
+Inductive v_pset A := v_PSet
+  { v_unPSet : dom (A ⇒ prop) }.
+Arguments v_PSet {A} _.
+Arguments v_unPSet {A} _.
+
+Definition pset A := derive (v_pset A) v_unPSet.
+
+Definition PSet {A} : dom ((A ⇒ prop) ⇒ pset A) := λ f →
+  v_PSet f : dom (pset A).
+Definition unPSet {A} : dom (pset A ⇒ A ⇒ prop) := λ aM →
+  v_unPSet (aM : dom (pset A)).
+
+Definition sempty {A} : dom (pset A) := undefined.
+Definition suniversal {A} : dom (pset A) := undefined.
+Definition ssingleton {A} : dom (A ⇒ pset A) := undefined.
+Definition sunion {A} : dom (pset A ⇒ pset A ⇒ pset A) := undefined.
+Definition sintersection {A} : dom (pset A ⇒ pset A ⇒ pset A) := undefined.
+
+Definition sinsert {A} : dom (A ⇒ pset A ⇒ pset A) := λ x → sunion ∙ (ssingleton ∙ x).
+
+Instance : forall A, Lattice (pset A).
+Admitted.
+Definition pset_bind {A B} : dom (pset A ⇒ (A ⇒ pset B) ⇒ pset B) := λ aM k → PSet $ λ b → all $ λ a → 
+  imp ∙ (unPSet ∙ aM ∙ a) ∙ (unPSet ∙ (k ∙ a) ∙ b).
+  
+Instance : Monad pset :=
+  { ret := @ssingleton 
+  ; bind := @pset_bind 
+  }.
+Admitted.
+Instance : MonadPlus pset :=
+  { mzero := @sempty
+  ; mplus := @sunion
+  }.
+Admitted.
