src/FP/Data/Prop.v
@@ -1,3 +1,12 @@
 Require Import FP.Core.
 
-Definition qprop := lib Prop.
+Instance : Eqv Prop := { eqv p q := p <-> q }.
+Admitted.
+
+Instance : Lte Prop := { lte p q := p -> q }.
+Admitted.
+
+Definition prop := {| qdom := Prop |}.
+Definition all {A} : dom ((A ⇒ prop) ⇒ prop) := λ f →
+  (forall (x:dom A), (f ∙ x : dom prop)) : dom prop.
+Definition imp : dom (prop ⇒ prop ⇒ prop) := λ p q → (p:dom prop) -> (q:dom prop) : dom prop.
