src/FP/Data/Stream.v
@@ -1,0 +1,13 @@
+Require Import FP.Core.
+
+Inductive v_step S A :=
+  | v_Done : v_step S A
+  | v_Yield : A -> S -> v_step S A.
+
+Inductive v_stream A := v_Stream
+  { v_streamS : Type
+  ; v_streamSeed : v_streamS
+  ; v_streamStep : v_step v_streamS A
+  }.
+
+Definition stream (A:qtype) := lib (v_stream (dom A)).
