src/FP/Data/WF.v
@@ -1,0 +1,164 @@
+Require Import FP.Core.
+Require Import FP.Data.Nat.
+Require Import FP.Classes.Monad.
+Require Import FP.Classes.Injection.
+Require Import FP.Classes.Lattice.
+Require Import FP.Classes.Injection.
+
+Definition wf_nat_lte {m:qtype -> qtype} {A} 
+: relation (dom nat -> dom (m A)) := fun f g => forall m, exists n, f m ⊑ g n.
+Definition wf_nat_eqv {m:qtype -> qtype} {A} 
+: relation (dom nat -> dom (m A)) := fun x y => wf_nat_lte x y /\ wf_nat_lte y x.
+
+Inductive v_wfT (m:qtype -> qtype) A := v_WfT
+  { v_unWfT : dom (nat ⇒ m A) }.
+Arguments v_WfT {m A} _.
+Arguments v_unWfT {m A} _.
+
+Definition wfT m A := derive (v_wfT m A) v_unWfT.
+
+Definition WfT {m A} : dom ((nat ⇒ m A) ⇒ wfT m A) := λ f → v_WfT f : dom (wfT m A).
+Definition unWfT {m A} : dom (wfT m A ⇒ nat ⇒ m A) := λ aM → v_unWfT (aM : dom (wfT m A)).
+Global Opaque WfT.
+Global Opaque unWfT.
+
+Instance : forall m A, InjectionEqv (@unWfT m A) :=
+  { injectionEqv _x _y p := p }.
+Instance : forall m A, InjectionLte (@unWfT m A) :=
+  { injectionLte _x _y p := p }.
+Definition WfT_inv {m A} (f:dom (nat ⇒ m A)) 
+: unWfT ∙ (WfT ∙ f) ≃ f := libReflexivity.
+Ltac WfTRewrite :=
+  match goal with
+  | |- ⟨ unWfT ∙ (WfT ∙ ?f) ∙ ?x IN ?k |?m| ?y ⟩ => change ⟨ f ∙ x IN k |m| y ⟩
+  | |- ⟨ unWfT ∙ (WfT ∙ ?f) IN _ |_| _ ⟩ => ReplaceBy (WfT_inv f)
+  end.
+
+Definition wfT_ret {m} `{! Monad m } {A} : dom (A ⇒ wfT m A) := λ x → WfT $ λ _ → ret ∙ x.
+Definition wfT_bind {m} `{! Monad m } {A B} : dom (wfT m A ⇒ (A ⇒ wfT m B) ⇒ wfT m B) := λ aM k →
+  WfT $ λ n →
+    a ← unWfT ∙ aM ∙ n ;;
+    unWfT ∙ (k ∙ a) ∙ n.
+Instance : forall m `{! Monad m }, Monad (wfT m) :=
+  { ret := @wfT_ret _ _
+  ; bind := @wfT_bind _ _
+  }. admit. admit. admit. Defined.
+Definition wfT_mret {m} `{! Monad m } {A} : dom (m A ⇒ wfT m A) := λ aM → WfT $ λ _ → aM.
+Instance : MonadRet wfT :=
+  { mret := @wfT_mret }.
+Instance : forall m `{! Monad m ,! MonadPlus m }, MonadPlus (wfT m).
+Admitted.
+
+Definition wfT_fix {m A} `{! Monad m ,! MonadPlus m } : dom ((A ⇒ wfT m A) ⇒ wfT m A) := 
+  λ f → WfT $ λ n →
+  (fix loop n :=
+    match n with
+    | O => mzero
+    | Coq.Init.Datatypes.S n' => 
+        x ← loop n' ;;
+        unWfT ∙ (f ∙ x) ∙ n 
+    end) (n:dom nat).
+Definition wfT_fix_beta_Z {m A} `{! Monad m ,! MonadPlus m } (f:dom (A ⇒ wfT m A)) 
+: unWfT ∙ (wfT_fix ∙ f) ∙ Z ≃ mzero := libReflexivity.
+Definition wfT_fix_beta_S {m A} `{! Monad m ,! MonadPlus m } (f:dom (A ⇒ wfT m A)) (n:dom nat)
+: unWfT ∙ (wfT_fix ∙ f) ∙ (S ∙ n) ≃ (x ← unWfT ∙ (wfT_fix ∙ f) ∙ n ;; unWfT ∙ (f ∙ x) ∙ (S ∙ n)) := libReflexivity.
+
+(*
+Definition wfT_eqv_intro {m A} (f g:dom nat -> dom (m A)) (p:wf_nat_eqv f g) : WFT_unsafe f ≃ WFT_unsafe g := p.
+Definition wfT_eqv_elim {m A} (f g:dom nat -> dom (m A)) (p:WFT_unsafe f ≃ WFT_unsafe g) : wf_nat_eqv f g := p.
+
+Definition wfT_lte_intro {m A} (f g:dom nat -> dom (m A)) (p:wf_nat_lte f g) : WFT_unsafe f ⊑ WFT_unsafe g := p.
+Definition wfT_lte_elim {m A} (f g:dom nat -> dom (m A)) (p:WFT_unsafe f ⊑ WFT_unsafe g) : wf_nat_lte f g := p.
+*)
+
+Definition later {m A} : dom (wfT m A ⇒ wfT m A) := λ aM → WfT $ λ n →
+  unWfT ∙ aM ∙ (pred ∙ n).
+
+Section Beta.
+
+  Definition wfT_fix_beta {m A} `{! Monad m ,! MonadPlus m } (f:dom (A ⇒ wfT m A)) 
+  : wfT_fix ∙ f ≃ (f =<< later ∙ (wfT_fix ∙ f)).
+  Proof.
+    unfold later,extend.
+    Local Transparent bind.
+    unfold bind.
+    Local Opaque bind.
+    simpl.
+    apply (injectionEqv unWfT).
+    apply qproper_intro ; unfold respectful ; intros ; simpl.
+    Re fail || WfTRewrite.
+    Re fail || match goal with |- ⟨ x IN _ |_| _ ⟩ => ReplaceBy H end.
+    clear x H.
+    nat_induction y ; Re fail || NatRewrite || MonadRewrite.
+    - Local Transparent wfT_fix.
+      unfold wfT_fix.
+      Local Opaque wfT_fix.
+      Re fail || WfTRewrite.
+      Local Transparent Z.
+      unfold Z.
+      Local Opaque Z.
+      Re fail || MonadPlusRewrite.
+    - Re fail || MonadRewrite.
+    Local Transparent bind.
+    unfold bind at 2.
+    Local Opaque bind.
+    Re fail || WfTRewrite.
+    nat_induction x.
+    - Re fail || WfTRewrite || NatRewrite.
+      Local Transparent Z.
+      unfold Z.
+      Local Opaque Z.
+      Re fail || MonadPlusRewrite.
+    - Local Transparent bind.
+      unfold bind at 3.
+      Local Opaque bind.
+      Re fail || WfTRewrite || NatRewrite.
+      eapply IHx.
+      cbv
+      simpl.
+      Symmetry.
+      EnterLeft.
+      match goal with |- ⟨ unWfT ∙ (WfT ∙ ?f) ∙ ?x IN ?k |EQV| ?y ⟩ => change ⟨ f ∙ x IN k |EQV| y ⟩ end.
+      PushArg.
+
+      Re fail || WfTRewrite.
+
+      EnterRight. 
+      WfTRewrite.
+      Re fail || WfTRewrite.
+    qproper_elim.
+    appl
+    match goal with
+    |- ?x ≃ ?y => Transitivity (WFT_unsafe (v_unWFT y))
+    end.
+    - Local Transparent bind.
+      Local Transparent mret.
+      simpl.
+      Local Opaque bind.
+      Local Opaque mret.
+      apply wfT_eqv_intro ; unfold wf_nat_eqv,wf_nat_lte ; split ; intros.
+      + exists m0.
+        induction m0.
+        * admit.
+        * EnterLeft ; PushFun ; PushArg.
+            WeakenBy IHm0.
+          PopArg ; PopFun ; ExitLeft.
+          Re fail || MonadRewrite.
+          admit.
+      + exists (Coq.Init.Datatypes.S m0).
+        Re fail || MonadRewrite.
+        admit.
+    - admit.
+  Qed.
+End Beta.
+
+Definition wfProp := dom nat -> Prop.
+
+Definition wf_lte {m} `{! Monad m } {A} (x:dom (wfT m A)) (y:dom (wfT m A)) : wfProp := fun m => exists n, v_unWFT x m ⊑ v_unWFT y n.
+
+Definition wf_eqv {m} `{! Monad m } {A} (x:dom (wfT m A)) (y:dom (wfT m A)) : wfProp := fun n => wf_lte x y n /\ wf_lte y x n.
+
+Definition wfDen : wfProp -> Prop := fun p => forall n, p n.
+
+Goal forall m A `{! Monad m } (xM yM:dom (wfT m A)), (wfDen (wf_eqv xM yM)) -> xM ≃ yM.
+Admitted.
