src/FP/Core/Notation.v
@@ -1,0 +1,50 @@
+Reserved Notation "v[ x , .. , y ]".
+Reserved Notation "⊤".
+Reserved Notation "⊥".
+
+Reserved Infix "∙" (at level 21, left associativity).
+
+Reserved Infix "⊔" (at level 45, right associativity).
+Reserved Infix "⊓" (at level 45, right associativity).
+
+Reserved Infix "⊙" (at level 51, right associativity).
+Reserved Infix "m⊙" (at level 51, right associativity).
+
+Reserved Infix "∷" (at level 55, right associativity).
+Reserved Infix "v∷" (at level 55, right associativity).
+
+Reserved Infix ">>=" (at level 61, left associativity).
+Reserved Infix "=<<" (at level 62, right associativity).
+
+Reserved Infix "m+" (at level 71, right associativity).
+
+Reserved Infix ",," (at level 79, right associativity).
+
+Reserved Infix "≃" (at level 81, no associativity).
+Reserved Infix "≄" (at level 81, no associativity).
+Reserved Infix "⊑" (at level 81, no associativity).
+Reserved Infix "⇉" (at level 81, right associativity).
+Reserved Infix "v⇉" (at level 81, right associativity).
+Reserved Infix "∈" (at level 81, right associativity).
+Reserved Infix "∉" (at level 81, right associativity).
+
+Reserved Infix "×" (at level 81, right associativity).
+Reserved Infix "v×" (at level 81, right associativity).
+
+Reserved Infix "⇒" (at level 86, right associativity).
+
+
+Reserved Notation "x ` f ` y" (at level 98, f at next level, right associativity).
+Reserved Notation "x v` f ` y" (at level 98, f at next level, right associativity).
+Reserved Infix "$" (at level 99, right associativity).
+Reserved Infix "v$" (at level 99, right associativity).
+
+Reserved Notation "x ← e₁  ;; e₂" (at level 100, e₁ at next level, right associativity).
+Reserved Infix ";;" (at level 100, right associativity).
+
+Reserved Notation "'λ'  x .. y → e" (at level 101, x binder, y binder, right associativity).
+
+Reserved Notation "⊤κ".
+Reserved Infix "◁" (at level 81, right associativity).
+Reserved Infix "▷" (at level 81, right associativity).
+Reserved Notation "⟨ x 'IN' k | m | y ⟩".
